theories/examples/swap_pair.v
@@ -7,7 +7,7 @@ From melocoton.lang_to_mlang Require Import lang weakestpre.
 From melocoton.interop Require Import lang weakestpre update_laws wp_utils wp_ext_call_laws wp_simulation.
 From melocoton.c_interop Require Import rules.
 From melocoton.ml_lang Require Import notation lang_instantiation.
-From melocoton.c_lang Require Import lang_instantiation.
+From melocoton.c_lang Require Import mlang_instantiation lang_instantiation.
 From melocoton.ml_lang Require proofmode.
 From melocoton.c_lang Require notation proofmode.
 From melocoton.mlanguage Require Import progenv.
@@ -23,7 +23,7 @@ Context `{!heapGS_C Σ, !heapGS_ML Σ, !invGS_gen hlc Σ, !primitive_laws.heapGS
 
 
 Definition swap_pair_code (x : expr) : expr :=
-  let: "lv" := malloc (#2) in 
+  let: "lv" := malloc (#2) in
   ("lv" +ₗ #0 <- (call: &"readfield" with (x, Val #0))) ;;
   ("lv" +ₗ #1 <- (call: &"readfield" with (x, Val #1))) ;;
   (call: &"registerroot" with ( Var "lv" +ₗ #0 )) ;;
@@ -37,83 +37,58 @@ Definition swap_pair_code (x : expr) : expr :=
   "np".
 
 Definition swap_pair_func : function := Fun [BNamed "x"] (swap_pair_code "x").
-
-Definition swap_pair_mod : gmap string function := {[ "swap_pair" := swap_pair_func ]}.
+Definition swap_pair_prog : lang_prog C_lang := {[ "swap_pair" := swap_pair_func ]}.
 
 Definition swap_pair_ml_spec : protocol ML_lang.val Σ := (
   λ s l wp, ∃ v1 v2, ⌜s = "swap_pair"⌝ ∗ ⌜l = [ (v1,v2)%MLV ]⌝ ∗ wp ((v2,v1)%MLV)
 )%I.
 
-Definition swap_pair_env : language.progenv.prog_environ C_lang Σ :=
-  ⟨ swap_pair_mod, (proto_prims_in_C ∅ swap_pair_ml_spec) ⟩.
-
-Lemma swap_pair_correct E f vs Φ :
-    wrap_proto swap_pair_ml_spec f vs Φ
- -∗ ∃ x, ⌜vs = [x]⌝ ∗ WP swap_pair_code (Val x) @ swap_pair_env; E {{a, Φ a }}.
+Lemma swap_pair_correct E :
+  wrap_proto swap_pair_ml_spec ⊑
+  prog_proto E swap_pair_prog (prims_proto ∅ ⊥).
 Proof.
-  iIntros "H". iNamed "H".
+  iIntros (fn ws Φ) "H". iNamed "H".
   iDestruct "Hproto" as (v1 v2) "(->&->&Hψ)".
-  rewrite /of_call /of_class /=.
-  unfold block_sim_arr.
-  iPoseProof (big_sepL2_cons_inv_l with "Hsim") as "(%l&%lr&->&Hsim&HsimL')".
-  iPoseProof (big_sepL2_nil_inv_l with "HsimL'") as "->".
-  cbn. iDestruct "Hsim" as "(%γpair&%lv1&%lv2&->&#Hptpair&#Hlv1&#Hlv2)".
-  destruct (Forall2_cons_inv_l _ _ _ _ Hrepr) as (w&aa'&Hγw&HH&Hx).
-  pose proof (Forall2_nil_inv_l _ _ HH); subst aa'. simplify_eq. clear HH Hrepr.
-  unfold swap_pair_code.
-  iExists _; iSplit; first done.
-  wp_alloc rr as "H". 1: done.
+  rewrite /prog_proto lookup_insert.
+  iAssert (⌜length lvs = 1⌝)%I with "[Hsim]" as %Hlen.
+  { by iDestruct (big_sepL2_length with "Hsim") as %?. }
+  destruct lvs as [|lv []]; try by (exfalso; eauto with lia); []. clear Hlen.
+  destruct ws as [|w []]; try by (exfalso; apply Forall2_length in Hrepr; eauto with lia); [].
+  apply Forall2_cons_1 in Hrepr as [Hrepr _].
+  iExists _. iSplit; first done. iNext.
+  iPoseProof (big_sepL2_cons_inv_l with "Hsim") as (l lr ?) "[Hsim _]".
+  simplify_eq.
+
+  wp_pures.
+  wp_alloc rr as "H"; first done.
   change (Z.to_nat 2) with 2. cbn. iDestruct "H" as "(H1&H2&_)". destruct rr as [rr].
   wp_pures.
 
-
   (* readfield 1 *)
-  wp_extern. cbn.
-  iModIntro. (iExists _; iSplit; first (iPureIntro; econstructor)).
-  iExists _, _, _, _, _, _, _, _. unfold named. iFrame "HGC".
-  do 2 (iSplitR; first done). iFrame "Hptpair".
-  do 2 (iSplitR; first done).
-  iIntros "!>" (v wlv1) "HGC #Helem1". change (Z.to_nat 0) with 0. cbn -[lstore_own_elem].
-  iIntros (Heq Hrepr1); injection Heq; intros <-. clear Heq.
-  wp_store.
+  iDestruct "Hsim" as (γ lv1 lv2 ->) "(#Hptpair & #Hlv1 & #Hlv2)".
+  wp_apply (wp_readfield with "[$HGC $Hptpair]"); [done..|].
+  iIntros (v wlv1) "(HGC & _ & %Heq & %Hrepr1)".
+  change (Z.to_nat 0) with 0 in Heq. cbn in *. symmetry in Heq. simplify_eq.
+  wp_store. wp_pures.
 
   (* readfield 2 *)
-  wp_pures.
-  wp_extern. cbn.
-  iModIntro. (iExists _; iSplit; first (iPureIntro; econstructor)).
-  iExists _, _, _, _, _, _, _, _. unfold named. iFrame "HGC".
-  do 2 (iSplitR; first done). iFrame "Hptpair".
-  do 2 (iSplitR; first done).
-  iIntros "!>" (v wlv2) "HGC #Helem2". change (Z.to_nat 1) with 1. cbn -[lstore_own_elem].
-  iIntros (Heq Hrepr2); injection Heq; intros <-. clear Heq.
-  wp_store.
+  wp_apply (wp_readfield with "[$HGC $Hptpair]"); [done..|].
+  iIntros (v wlv2) "(HGC & _ & %Heq & %Hrepr2)".
+  change (Z.to_nat 1) with 1 in Heq. cbn in *. symmetry in Heq. simplify_eq.
+  wp_store. wp_pures.
 
   (* registerroot 1 *)
-  wp_pures.
-  wp_extern. cbn.
-  iModIntro. (iExists _; iSplit; first (iPureIntro; econstructor)).
-  iExists _, _, _, _. unfold named. iFrame "HGC".
-  iSplitR; first done. iSplitL "H1"; first done.
-  iSplitR; first done.
-  iIntros "!> HGC H1r".
+  wp_apply (wp_registerroot with "[$HGC $H1]"); [done..|].
+  iIntros "(HGC & H1r)". wp_pures.
 
   (* registerroot 2 *)
-  wp_pures.
-  wp_extern. cbn.
-  iModIntro. (iExists _; iSplit; first (iPureIntro; econstructor)).
-  iExists _, _, _, _. unfold named. iFrame "HGC".
-  iSplitR; first done. iSplitL "H2"; first done.
-  iSplitR; first done.
-  iIntros "!> HGC H2r".
+  wp_apply (wp_registerroot with "[$HGC $H2]"); [done..|].
+  iIntros "(HGC & H2r)". wp_pures.
 
   (* alloc *)
-  wp_pures.
-  wp_extern. cbn.
-  iModIntro. (iExists _; iSplit; first (iPureIntro; econstructor)).
-  iExists _, TagDefault, _. unfold named. iFrame "HGC".
-  do 2 (iSplitR; first done).
-  iIntros "!>" (θ' γnew wnew) "HGC Hnew %Hreprnew".
-  wp_pures. change (Z.to_nat 2) with 2. cbn.
+  wp_apply (wp_alloc _ _ _ _ TagDefault with "HGC"); [done..|].
+  iIntros (θ' γnew wnew) "(HGC & Hnew & %Hreprnew)".
+  wp_pures. change (Z.to_nat 2) with 2. cbn [repeat].
 
   (* load from root *)
   wp_bind (Load _).
@@ -121,54 +96,36 @@ Proof.
   iIntros (wlv1') "(Hr1&HGC&%Hrepr1')".
 
   (* modify 1 *)
+  wp_apply (wp_modify with "[$HGC $Hnew]"); [done..|].
+  iIntros "(HGC & Hnew)". change (Z.to_nat 1) with 1. cbn.
   wp_pures.
-  wp_extern. cbn.
-  iModIntro. (iExists _; iSplit; first (iPureIntro; econstructor)).
-  do 9 iExists _. unfold named. iFrame "HGC Hnew".
-  do 6 (iSplitR; first done).
-  iIntros "!> HGC Hnew1". change (Z.to_nat 1) with 1. cbn.
 
   (* load from root *)
-  wp_pures. wp_bind (Load _).
+  wp_bind (Load _).
   wp_apply (load_from_root with "[HGC H2r]"); first iFrame.
   iIntros (wlv2') "(Hr2&HGC&%Hrepr2')".
 
   (* modify 2 *)
+  wp_apply (wp_modify with "[$HGC $Hnew]"); [done..|].
+  iIntros "(HGC & Hnew)". change (Z.to_nat 0) with 0. cbn.
   wp_pures.
-  wp_extern. cbn.
-  iModIntro. (iExists _; iSplit; first (iPureIntro; econstructor)).
-  do 9 iExists _. unfold named. iFrame "HGC Hnew1".
-  do 6 (iSplitR; first done).
-  iIntros "!> HGC Hnew1". change (Z.to_nat 0) with 0. cbn.
 
   (* unregisterroot 1 *)
-  wp_pures.
-  wp_extern. cbn.
-  iModIntro. (iExists _; iSplit; first (iPureIntro; econstructor)).
-  iExists _, _, _. unfold named. iFrame "HGC Hr1".
-  iSplitR; first done.
-  iIntros "!>" (wlv1'') "HGC Hr1 %Hrepr1'1".
-  destruct (repr_lval_inj _ _ _ _ Hrepr1' Hrepr1'1). (* ugly subst*) 
-  clear Hrepr1'1.
+  wp_apply (wp_unregisterroot with "[$HGC $Hr1]"); [done..|].
+  iIntros (wlv1'') "(HGC & H1 & %Hrepr1'1)".
+  repr_lval_inj. wp_pures.
 
   (* unregisterroot 2 *)
-  wp_pures.
-  wp_extern. cbn.
-  iModIntro. (iExists _; iSplit; first (iPureIntro; econstructor)).
-  iExists _, _, _. unfold named. iFrame "HGC Hr2".
-  iSplitR; first done.
-  iIntros "!>" (wlv2'') "HGC Hr2 %Hrepr2'1".
-  destruct (repr_lval_inj _ _ _ _ Hrepr2' Hrepr2'1). (* ugly subst*)
-  clear Hrepr2'1.
+  wp_apply (wp_unregisterroot with "[$HGC $Hr2]"); [done..|].
+  iIntros (wlv2'') "(HGC & H2 & %Hrepr2'1)".
+  repr_lval_inj. wp_pures.
 
   (* free *)
-  wp_pures.
-  iAssert ((Loc rr) ↦C∗ [Some wlv1'; Some wlv2'])%I with "[Hr1 Hr2]" as "Hrr".
+  iAssert ((Loc rr) ↦C∗ [Some wlv1'; Some wlv2'])%I with "[H1 H2]" as "Hrr".
   1: cbn; iFrame.
-  wp_free.
+  wp_free. wp_pures.
 
-  (* Finish, convert points-to *)
-  wp_pures.
+  (* Finish, convert the new points-to to an immutable pointsto *)
   iMod (freeze_to_immut γnew _ θ' with "[$]") as "(HGC&#Hnew)".
 
   iModIntro. iApply ("Cont" with "HGC Hψ [] []").
@@ -185,13 +142,12 @@ Import melocoton.ml_lang.proofmode.
 
 Context `{!heapGS_C Σ, !invGS_gen hlc Σ, !heapGS_ML Σ, !wrapperGS Σ, !linkGS Σ}.
 
-Definition swap_pair_client : mlanguage.expr (lang_to_mlang ML_lang) := 
+(* TODO: define ML_mlang? *)
+Definition swap_pair_client : mlanguage.expr (lang_to_mlang ML_lang) :=
   (Extern "swap_pair" [ ((#3, (#1, #2)))%MLE ]).
 
-Definition client_env : prog_environ ML_lang Σ := ⟨ ∅, swap_pair_ml_spec ⟩.
-Definition client_env_wrapped := ⟪ prims_prog, wrap_proto swap_pair_ml_spec ⟫.
-
-Lemma ML_prog_correct_axiomatic E : ⊢ WP swap_pair_client @ client_env ; E {{v, ⌜v = (#1,#2,#3)⌝%MLV}}.
+Lemma ML_prog_correct_axiomatic E :
+  ⊢ WP swap_pair_client @ ⟨∅, swap_pair_ml_spec⟩ ; E {{v, ⌜v = (#1,#2,#3)⌝%MLV}}.
 Proof.
   iStartProof. unfold swap_pair_client. wp_pures.
   wp_extern.
@@ -202,59 +158,26 @@ Qed.
 
 Import melocoton.mlanguage.weakestpre.
 
-Notation combined_lang := (link_lang wrap_lang (lang_to_mlang C_lang)).
-Definition swap_pair_env_lifted := penv_to_mlang swap_pair_env.
-
-Lemma swap_pair_correct_lifted E f vs Φ :
-    wrap_proto swap_pair_ml_spec f vs Φ
- -∗ ∃ x, ⌜vs = [x]⌝ ∗ WP (swap_pair_code (C_lang.Val x) : expr (lang_to_mlang (C_lang))) @ swap_pair_env_lifted ; E {{a, Φ a }}.
+Lemma is_linkable_swap_pair :
+  can_link wrap_lang C_mlang
+    prims_prog (wrap_proto swap_pair_ml_spec)
+    swap_pair_prog (prims_proto ∅ ⊥)
+    ⊥.
 Proof.
-  iIntros "H".
-  iPoseProof (swap_pair_correct with "H") as (x ->) "HWP".
-  iExists _; iSplit; first done.
-  by iApply wp_lang_to_mlang.
-Qed.
-
-Definition linked_env : prog_environ combined_lang Σ :=
-  ⟪ fmap inl prims.prims_prog ∪ fmap inr swap_pair_mod, ⊥ ⟫.
-
-Lemma is_linkable_swap_pair : is_link_environ client_env_wrapped swap_pair_env_lifted linked_env.
-Proof.
-  split.
+  constructor; intros.
   - rewrite !dom_insert_L !dom_empty_L. set_solver.
-  - done.
-  - cbn. unfold swap_pair_mod.
-    iIntros (fn F vs Φ E [<- <-]%lookup_singleton_Some) "HH".
-    iPoseProof (swap_pair_correct_lifted with "HH") as (w ->) "HWP".
-    rewrite /C_lang.apply_function /swap_pair_func.
-    cbn -[C_lang.subst_all].
-    iExists _; iSplit; first done.
-    iNext. iIntros "Hbound". iApply (wp_wand with "[HWP]").
-    { solve_lookup_fixed; iApply "HWP". }
-    iIntros (v) "H". iFrame.
-  - iIntros (fname func vs Φ E Hfunc) "Hproto".
-    iExists _; iSplit; first done.
-    iApply bi.later_intro.
-    iIntros "Hb". iApply (@wp_wand with "[Hb Hproto]");
-    first iApply (wp_primitive with "[] [Hproto]").
-    + iIntros (fn_name vs' Φ' Hprims) "HH".
-      cbn. iDestruct "HH" as "(%&%&->&_)". inversion Hprims. inversion H. 
-    + cbn. iDestruct "Hproto" as "(%pr&%HH1&HH2)".
-      apply prims.lookup_prims_prog_Some in Hfunc.
-      pose proof (prims.is_prim_inj _ _ _ HH1 Hfunc) as ->.
-      iApply proto_prim_mask_mono; last done.
-      apply namespaces.coPset_empty_subseteq.
-    + done.
-    + iIntros (v) "(Hb&Hv)". iFrame.
-  - iIntros (fn vs Φ HH1 HH2) "H". iNamed "H".
-    iDestruct "Hproto" as (v1 v2 -> ->) "H".
-    rewrite lookup_insert in HH2; done.
-  - iIntros (fn vs Φ HH1 HH2) "H".
-    rewrite /=. iDestruct "H" as (prim HH%prims.lookup_prims_prog_Some) "H".
-    rewrite HH in HH1. done.
+  - rewrite proto_on_refines swap_pair_correct lang_to_mlang_refines //.
+  - rewrite proto_on_refines prims_proto_refines.
+    2: { rewrite proto_on_refines //. }
+    eapply mprog_proto_mono; first set_solver.
+    apply wrap_proto_mono, proto_refines_bot_l.
+  - iIntros (? ? ?) "H". rewrite /proto_except.
+    iDestruct "H" as (?) "H". iNamed "H".
+    iDestruct "Hproto" as (? ? ->) "H". set_solver.
+  - apply prims_proto_except_dom.
 Qed.
 
-Notation link_in_state := (link_in_state wrap_lang (lang_to_mlang C_lang)).
+Notation link_in_state := (link_in_state wrap_lang C_mlang).
 (*
 Lemma linked_prog_correct_overall E : 
     link_in_state In1
