theories/linking/weakestpre.v
@@ -22,8 +22,8 @@ Context {Σ : gFunctors}.
 Context {val pubstate : Type}.
 Context (Λ1 Λ2 : mlanguage val).
 Context `{!linkGS Σ}.
-Context `{!mlangGS val Σ Λ1}.
-Context `{!mlangGS val Σ Λ2}.
+Context `{!mlangGS val Λ1 Σ}.
+Context `{!mlangGS val Λ2 Σ}.
 Context `{!invGS_gen hlc Σ}.
 Context (public_state_interp : pubstate → iProp Σ).
 Context `{!linkable Λ1 pubstate}.
@@ -97,7 +97,7 @@ Proof using.
   all: by iDestruct (ghost_var_agree with "Hb Hb'") as %?.
 Qed.
 
-Global Program Instance link_mlangGS : mlangGS val Σ (link_lang Λ1 Λ2) := {
+Global Program Instance link_mlangGS : mlangGS val (link_lang Λ1 Λ2) Σ := {
   state_interp := link_state_interp;
   at_boundary := link_in_state Boundary;
 }.
@@ -121,61 +121,48 @@ Next Obligation.
   iPureIntro. eexists _, _. constructor.
 Qed.
 
-Lemma proj1_prog_union (pe1: mlanguage.prog Λ1) (pe2: mlanguage.prog Λ2) :
-  dom pe1 ## dom pe2 →
-  Link.proj1_prog _ _ (fmap inl pe1 ∪ fmap inr pe2) = pe1.
+Definition link_prog
+  (p1 : mlang_prog Λ1) (p2 : mlang_prog Λ2) :
+  mlang_prog (link_lang Λ1 Λ2)
+:=
+  fmap inl p1 ∪ fmap inr p2.
+
+Lemma proj1_prog_union (p1: mlanguage.prog Λ1) (p2: mlanguage.prog Λ2) :
+  dom p1 ## dom p2 →
+  Link.proj1_prog _ _ (link_prog p1 p2) = p1.
 Proof using.
   intros Hdisj.
   apply map_eq. intros fname. unfold Link.proj1_prog.
   rewrite map_omap_union.
   2: { apply map_disjoint_dom. rewrite !dom_fmap//. }
   rewrite lookup_union_l.
-  { rewrite lookup_omap /= lookup_fmap. by destruct (pe1 !! fname). }
-  { rewrite lookup_omap /= lookup_fmap. by destruct (pe2 !! fname). }
+  { rewrite lookup_omap /= lookup_fmap. by destruct (p1 !! fname). }
+  { rewrite lookup_omap /= lookup_fmap. by destruct (p2 !! fname). }
 Qed.
 
-Lemma proj2_prog_union (pe1: mlanguage.prog Λ1) (pe2: mlanguage.prog Λ2) :
-  dom pe1 ## dom pe2 →
-  Link.proj2_prog _ _ (fmap inl pe1 ∪ fmap inr pe2) = pe2.
+Lemma proj2_prog_union (p1: mlanguage.prog Λ1) (p2: mlanguage.prog Λ2) :
+  dom p1 ## dom p2 →
+  Link.proj2_prog _ _ (link_prog p1 p2) = p2.
 Proof using.
   intros Hdisj.
   apply map_eq. intros fname. unfold Link.proj2_prog.
   rewrite map_omap_union.
   2: { apply map_disjoint_dom. rewrite !dom_fmap//. }
   rewrite lookup_union_r.
-  { rewrite lookup_omap /= lookup_fmap. by destruct (pe2 !! fname). }
-  { rewrite lookup_omap /= lookup_fmap. by destruct (pe1 !! fname). }
+  { rewrite lookup_omap /= lookup_fmap. by destruct (p2 !! fname). }
+  { rewrite lookup_omap /= lookup_fmap. by destruct (p1 !! fname). }
 Qed.
 
-Class is_link_environ
-  (pe1 : prog_environ Λ1 Σ) (pe2 : prog_environ Λ2 Σ)
-  (pe : prog_environ (link_lang Λ1 Λ2) Σ)
-:= IsLinkEnviron {
-  is_link_dom_disj : dom (penv_prog pe1) ## dom (penv_prog pe2);
-  is_link_prog : penv_prog pe = fmap inl (penv_prog pe1) ∪ fmap inr (penv_prog pe2);
-
-  is_link_internal1 fname (func: mlanguage.func Λ2) vs Φ E :
-    penv_prog pe2 !! fname = Some func →
-    penv_proto pe1 fname vs Φ -∗
-    ∃ e2, ⌜apply_func func vs = Some e2⌝ ∗ ▷
-      (at_boundary Λ2 -∗ WP e2 @ pe2; E {{
-        λ v, Φ v ∗ at_boundary Λ2 }});
-
-  is_link_internal2 fname (func: mlanguage.func Λ1) vs Φ E :
-    penv_prog pe1 !! fname = Some func →
-    penv_proto pe2 fname vs Φ -∗
-    ∃ e1, ⌜apply_func func vs = Some e1⌝ ∗ ▷
-      (at_boundary Λ1 -∗ WP e1 @ pe1; E {{
-        λ v, Φ v ∗ at_boundary Λ1 }});
-
-  is_link_external1 fname vs Φ :
-    penv_prog pe1 !! fname = None →
-    penv_prog pe2 !! fname = None →
-    penv_proto pe1 fname vs Φ -∗ penv_proto pe fname vs Φ;
-  is_link_external2 fname vs Φ :
-    penv_prog pe1 !! fname = None →
-    penv_prog pe2 !! fname = None →
-    penv_proto pe2 fname vs Φ -∗ penv_proto pe fname vs Φ;
+Class can_link
+  (p1 : mlang_prog Λ1) (Ψ1 : protocol val Σ)
+  (p2 : mlang_prog Λ2) (Ψ2 : protocol val Σ)
+  (Ψ : protocol val Σ)
+:= CanLink {
+  can_link_prog_disj : dom p1 ## dom p2;
+  can_link_internal1 E : Ψ1 on (dom p2) ⊑ mprog_proto E p2 Ψ2;
+  can_link_internal2 E : Ψ2 on (dom p1) ⊑ mprog_proto E p1 Ψ1;
+  can_link_external1 : Ψ1 except (dom p2) ⊑ Ψ;
+  can_link_external2 : Ψ2 except (dom p1) ⊑ Ψ;
 }.
 
 Lemma wp_link_call (pe : prog_environ (link_lang Λ1 Λ2) Σ) E k fn vs Φ fname :
@@ -193,23 +180,25 @@ Proof using.
   iPureIntro; eapply H4. done.
 Qed.
 
-Lemma wp_link_run_function_1 pe1 pe2 pe E k2 k fn arg fname Φ Ξ :
-  is_link_environ pe1 pe2 pe →
-  penv_prog pe1 !! fname = Some fn →
+Lemma wp_link_run_function_1 p1 p2 Ψ1 Ψ2 Ψ E k2 k fn arg fname Φ Ξ :
+  can_link p1 Ψ1 p2 Ψ2 Ψ →
+  p1 !! fname = Some fn →
   link_state_frag Boundary -∗
   at_boundary Λ1 -∗
-  penv_proto pe2 fname arg Ξ -∗
+  Ψ2 fname arg Ξ -∗
   (∀ e1, ⌜apply_func fn arg = Some e1⌝ -∗
-         WP e1 @ pe1; E {{ v, Ξ v ∗ at_boundary Λ1 }} -∗
+         WP e1 @ ⟪p1, Ψ1⟫; E {{ v, Ξ v ∗ at_boundary Λ1 }} -∗
          link_state_frag In1 -∗
-         WP Link.LkE (Link.Expr1 e1) (inr k2 :: k) @ pe; E {{ Φ }}) -∗
-  WP Link.LkE (Link.RunFunction (inl fn) arg) (inr k2 :: k) @ pe; E {{ Φ }}.
+         WP Link.LkE (Link.Expr1 e1) (inr k2 :: k) @ ⟪link_prog p1 p2, Ψ⟫; E {{ Φ }}) -∗
+  WP Link.LkE (Link.RunFunction (inl fn) arg) (inr k2 :: k) @ ⟪link_prog p1 p2, Ψ⟫; E {{ Φ }}.
 Proof using.
-  iIntros (Hislink Hfn) "Hb Hb1 HTΞ Hwp".
+  iIntros (Hcanlink Hfn) "Hb Hb1 HTΞ Hwp".
   iApply wp_unfold. rewrite /wp_pre.
   iIntros (σ) "Hσ". iDestruct (link_at_boundary with "Hσ Hb") as %(pubσ&privσ1&privσ2&->).
   iRight; iRight.
-  iPoseProof (is_link_internal2 _ _ _ _ E Hfn with "HTΞ") as (? Happlyfunc) "Hwpcall".
+  iPoseProof (can_link_internal2 _ _ _ with "[HTΞ]") as "H".
+  { rewrite /proto_on. iFrame. iPureIntro. by eapply elem_of_dom_2. }
+  rewrite /mprog_proto Hfn. iDestruct "H" as (? Happlyfunc) "Hwpcall".
   iDestruct "Hσ" as "(Hob & Hpubσ & Hprivσ1 & Hprivσ2)".
   iMod (state_interp_join with "Hpubσ Hprivσ1") as (σ1) "(Hσ1 & %Hsplit)". iModIntro.
   iSplit; first done.
@@ -219,26 +208,28 @@ Proof using.
   iMod (link_state_update _ In1 with "Hob Hb") as "(Hob & Hb)".
   iModIntro. iExists _, _. iSplitR; first by eauto. iFrame.
   iDestruct ("Hwpcall" with "Hb1") as "Hwpcall".
-  by iApply ("Hwp" with "[] Hwpcall Hob").
+  iApply ("Hwp" with "[] Hwpcall Hob"); first done.
 Qed.
 
-Lemma wp_link_run_function_2 pe1 pe2 pe E k1 k fn arg fname Φ Ξ :
-  is_link_environ pe1 pe2 pe →
-  penv_prog pe2 !! fname = Some fn →
+Lemma wp_link_run_function_2 p1 p2 Ψ1 Ψ2 Ψ E k1 k fn arg fname Φ Ξ :
+  can_link p1 Ψ1 p2 Ψ2 Ψ →
+  p2 !! fname = Some fn →
   link_state_frag Boundary -∗
   at_boundary Λ2 -∗
-  penv_proto pe1 fname arg Ξ -∗
+  Ψ1 fname arg Ξ -∗
   (∀ e2, ⌜apply_func fn arg = Some e2⌝ -∗
-         WP e2 @ pe2; E {{ v, Ξ v ∗ at_boundary Λ2 }} -∗
+         WP e2 @ ⟪p2, Ψ2⟫; E {{ v, Ξ v ∗ at_boundary Λ2 }} -∗
          link_state_frag In2 -∗
-         WP Link.LkE (Link.Expr2 e2) (inl k1 :: k) @ pe; E {{ Φ }}) -∗
-  WP Link.LkE (Link.RunFunction (inr fn) arg) (inl k1 :: k) @ pe; E {{ Φ }}.
+         WP Link.LkE (Link.Expr2 e2) (inl k1 :: k) @ ⟪link_prog p1 p2, Ψ⟫; E {{ Φ }}) -∗
+  WP Link.LkE (Link.RunFunction (inr fn) arg) (inl k1 :: k) @ ⟪link_prog p1 p2, Ψ⟫; E {{ Φ }}.
 Proof using.
-  iIntros (Hislink Hfn) "Hb Hb2 HTΞ Hwp".
+  iIntros (Hcanlink Hfn) "Hb Hb2 HTΞ Hwp".
   iApply wp_unfold. rewrite /wp_pre.
   iIntros (σ) "Hσ". iDestruct (link_at_boundary with "Hσ Hb") as %(pubσ&privσ1&privσ2&->).
   iRight; iRight.
-  iPoseProof (is_link_internal1 _ _ _ _ E Hfn with "HTΞ") as (? Happlyfunc) "Hwpcall".
+  iPoseProof (can_link_internal1 _ _ _ with "[HTΞ]") as "H".
+  { rewrite /proto_on. iFrame. iPureIntro. by eapply elem_of_dom_2. }
+  rewrite /mprog_proto Hfn. iDestruct "H" as (? Happlyfunc) "Hwpcall".
   iDestruct "Hσ" as "(Hob & Hpubσ & Hprivσ1 & Hprivσ2)".
   iMod (state_interp_join with "Hpubσ Hprivσ2") as (σ2) "(Hσ2 & %Hsplit)". iModIntro.
   iSplit; first done.
@@ -289,99 +280,101 @@ Proof using.
   iModIntro. iExists _, _. iSplitR; first by eauto. iFrame. iApply "Hwp". iFrame.
 Qed.
 
-Lemma wp_link_extcall_1 pe1 pe2 pe E k1 fn_name arg Φ Ξ :
-  is_link_environ pe1 pe2 pe →
-  penv_prog pe1 !! fn_name = None →
-  penv_prog pe2 !! fn_name = None →
-  penv_proto pe1 fn_name arg Ξ -∗
+Lemma wp_link_extcall_1 p1 p2 Ψ1 Ψ2 Ψ E k1 fn_name arg Φ Ξ :
+  can_link p1 Ψ1 p2 Ψ2 Ψ →
+  p1 !! fn_name = None →
+  p2 !! fn_name = None →
+  Ψ1 fn_name arg Ξ -∗
   (▷ ∀ r : val, Ξ r ∗ at_boundary Λ1 -∗
-        WP resume_with k1 (of_val Λ1 r) @ pe1; E {{ λ v, Φ v ∗ at_boundary Λ1 }}) -∗
-  (▷ ∀ r, WP resume_with k1 (of_val Λ1 r) @ pe1; E {{ λ v, Φ v ∗ at_boundary Λ1 }} -∗
+        WP resume_with k1 (of_val Λ1 r) @ ⟪p1, Ψ1⟫; E {{ λ v, Φ v ∗ at_boundary Λ1 }}) -∗
+  (▷ ∀ r, WP resume_with k1 (of_val Λ1 r) @ ⟪p1, Ψ1⟫; E {{ λ v, Φ v ∗ at_boundary Λ1 }} -∗
         link_state_frag Boundary -∗
         at_boundary Λ2 -∗
-        WP Link.LkE (Link.ExprV r) [inl k1] @ pe; E {{ λ v, Φ v ∗ at_boundary (link_lang Λ1 Λ2) }}) -∗
+        WP Link.LkE (Link.ExprV r) [inl k1] @ ⟪link_prog p1 p2, Ψ⟫; E {{ λ v, Φ v ∗ at_boundary (link_lang Λ1 Λ2) }}) -∗
   at_boundary (link_lang Λ1 Λ2) -∗
-  WP Link.LkE (Link.ExprCall fn_name arg) [inl k1] @ pe; E {{ λ v, Φ v ∗ at_boundary (link_lang Λ1 Λ2) }}.
+  WP Link.LkE (Link.ExprCall fn_name arg) [inl k1] @ ⟪link_prog p1 p2, Ψ⟫; E {{ λ v, Φ v ∗ at_boundary (link_lang Λ1 Λ2) }}.
 Proof using.
-  iIntros (Hislink Hfn1 Hfn2) "HTΞ HΞ Hwp (Hb & Hb1 & Hb2)".
-  assert (Hpef: penv_prog pe !! fn_name = None).
-  { rewrite is_link_prog. apply lookup_union_None. rewrite !lookup_fmap Hfn1 Hfn2 //. }
+  iIntros (Hcanlink Hfn1 Hfn2) "HTΞ HΞ Hwp (Hb & Hb1 & Hb2)".
   iApply wp_unfold. rewrite /wp_pre.
   iIntros (σ) "Hσ". iDestruct (link_at_boundary with "Hσ Hb") as %(pubσ&privσ1&privσ2&->).
   iModIntro. iRight; iLeft. iExists _, _, [inl k1]. iSplitR; [by eauto|].
-  iSplitR; first by eauto. iFrame "Hσ Hb Hb1 Hb2". iExists Ξ. iSplitL "HTΞ".
-  { by iApply is_link_external1. }
+  iSplit.
+  { iPureIntro. apply lookup_union_None. rewrite !lookup_fmap Hfn1 Hfn2 //. }
+  iFrame "Hσ Hb Hb1 Hb2". iExists Ξ. iSplitL "HTΞ".
+  { cbn. iApply can_link_external1. iFrame. iPureIntro.
+    by apply not_elem_of_dom_2. }
   iNext. iIntros (r) "[Hr Hb]". iDestruct "Hb" as "(Hb & Hb1 & Hb2)".
   simpl.
   iSpecialize ("HΞ" with "[$Hr $Hb1]").
   iApply ("Hwp" with "HΞ Hb Hb2").
 Qed.
 
-Lemma wp_link_extcall_2 pe1 pe2 pe E k2 fn_name arg Φ Ξ :
-  is_link_environ pe1 pe2 pe →
-  penv_prog pe1 !! fn_name = None →
-  penv_prog pe2 !! fn_name = None →
-  penv_proto pe2 fn_name arg Ξ -∗
+Lemma wp_link_extcall_2 p1 p2 Ψ1 Ψ2 Ψ E k2 fn_name arg Φ Ξ :
+  can_link p1 Ψ1 p2 Ψ2 Ψ →
+  p1 !! fn_name = None →
+  p2 !! fn_name = None →
+  Ψ2 fn_name arg Ξ -∗
   (▷ ∀ r : val, Ξ r ∗ at_boundary Λ2 -∗
-        WP resume_with k2 (of_val Λ2 r) @ pe2; E {{ λ v, Φ v ∗ at_boundary Λ2 }}) -∗
-  (▷ ∀ r, WP resume_with k2 (of_val Λ2 r) @ pe2; E {{ λ v, Φ v ∗ at_boundary Λ2 }} -∗
+        WP resume_with k2 (of_val Λ2 r) @ ⟪p2, Ψ2⟫; E {{ λ v, Φ v ∗ at_boundary Λ2 }}) -∗
+  (▷ ∀ r, WP resume_with k2 (of_val Λ2 r) @ ⟪p2, Ψ2⟫; E {{ λ v, Φ v ∗ at_boundary Λ2 }} -∗
         link_state_frag Boundary -∗
         at_boundary Λ1 -∗
-        WP Link.LkE (Link.ExprV r) [inr k2] @ pe; E {{ λ v, Φ v ∗ at_boundary (link_lang Λ1 Λ2) }}) -∗
+        WP Link.LkE (Link.ExprV r) [inr k2] @ ⟪link_prog p1 p2, Ψ⟫; E {{ λ v, Φ v ∗ at_boundary (link_lang Λ1 Λ2) }}) -∗
   at_boundary (link_lang Λ1 Λ2) -∗
-  WP Link.LkE (Link.ExprCall fn_name arg) [inr k2] @ pe; E {{ λ v, Φ v ∗ at_boundary (link_lang Λ1 Λ2) }}.
+  WP Link.LkE (Link.ExprCall fn_name arg) [inr k2] @ ⟪link_prog p1 p2, Ψ⟫; E {{ λ v, Φ v ∗ at_boundary (link_lang Λ1 Λ2) }}.
 Proof using.
-  iIntros (Hislink Hfn1 Hfn2) "HTΞ HΞ Hwp (Hb & Hb1 & Hb2)".
-  assert (Hpef: penv_prog pe !! fn_name = None).
-  { rewrite is_link_prog. apply lookup_union_None. rewrite !lookup_fmap Hfn1 Hfn2 //. }
+  iIntros (Hcanlink Hfn1 Hfn2) "HTΞ HΞ Hwp (Hb & Hb1 & Hb2)".
   iApply wp_unfold. rewrite /wp_pre.
   iIntros (σ) "Hσ". iDestruct (link_at_boundary with "Hσ Hb") as %(pubσ&privσ1&privσ2&->).
   iModIntro. iRight; iLeft. iExists _, _, [inr k2]. iSplitR; [by eauto|].
-  iSplitR; first by eauto. iFrame "Hσ Hb Hb1 Hb2". iExists Ξ. iSplitL "HTΞ".
-  { by iApply is_link_external2. }
+  iSplit.
+  { iPureIntro. apply lookup_union_None. rewrite !lookup_fmap Hfn1 Hfn2 //. }
+  iFrame "Hσ Hb Hb1 Hb2". iExists Ξ. iSplitL "HTΞ".
+  { cbn. iApply can_link_external2. iFrame. iPureIntro.
+    by apply not_elem_of_dom_2. }
   iNext. iIntros (r) "[Hr Hb]". iDestruct "Hb" as "(Hb & Hb1 & Hb2)".
   simpl.
   iSpecialize ("HΞ" with "[$Hr $Hb2]").
   iApply ("Hwp" with "HΞ Hb Hb1").
 Qed.
 
-Lemma link_step_call_ext_1_inv pe1 pe2 pe e C f vs σ1 pubσ privσ1 privσ2 X :
-  is_link_environ pe1 pe2 pe →
-  penv_prog pe1 !! f = None →
-  prim_step (penv_prog pe) (LkSE (Link.Expr1 e), Link.St1 σ1 privσ2) X →
+Lemma link_step_call_ext_1_inv p1 p2 Ψ1 Ψ2 Ψ e C f vs σ1 pubσ privσ1 privσ2 X :
+  can_link p1 Ψ1 p2 Ψ2 Ψ →
+  p1 !! f = None →
+  prim_step (link_prog p1 p2) (LkSE (Link.Expr1 e), Link.St1 σ1 privσ2) X →
   split_state σ1 pubσ privσ1 →
   is_call e f vs C →
   X (Link.LkE (Link.ExprCall f vs) [inl C], Link.St pubσ privσ1 privσ2).
-Proof.
+Proof using.
   intros Hlink Heq; inversion 1; simplify_eq /=; intros Hsplit Hiscall.
   eapply H5; try done.
-  rewrite is_link_prog proj1_prog_union; first done. apply Hlink.
+  rewrite proj1_prog_union; first done. apply Hlink.
 Qed.
 
 
-Lemma link_step_call_ext_2_inv pe1 pe2 pe e C f vs σ2 pubσ privσ1 privσ2 X :
-  is_link_environ pe1 pe2 pe →
-  penv_prog pe2 !! f = None →
-  prim_step (penv_prog pe) (LkSE (Link.Expr2 e), Link.St2 privσ1 σ2) X →
+Lemma link_step_call_ext_2_inv p1 p2 Ψ1 Ψ2 Ψ e C f vs σ2 pubσ privσ1 privσ2 X :
+  can_link p1 Ψ1 p2 Ψ2 Ψ →
+  p2 !! f = None →
+  prim_step (link_prog p1 p2) (LkSE (Link.Expr2 e), Link.St2 privσ1 σ2) X →
   split_state σ2 pubσ privσ2 →
   is_call e f vs C →
   X (Link.LkE (Link.ExprCall f vs) [inr C], Link.St pubσ privσ1 privσ2).
-Proof.
+Proof using.
   intros Hlink Heq; inversion 1; simplify_eq /=; intros Hsplit Hiscall.
   eapply H5; try done.
-  rewrite is_link_prog proj2_prog_union; first done. apply Hlink.
+  rewrite proj2_prog_union; first done. apply Hlink.
 Qed.
 
-Lemma wp_link_run_mut pe1 pe2 pe E :
-  is_link_environ pe1 pe2 pe →
+Lemma wp_link_run_mut p1 p2 Ψ1 Ψ2 Ψ E :
+  can_link p1 Ψ1 p2 Ψ2 Ψ →
   ⊢ □ (
-    (∀ e1 Φ, WP e1 @ pe1; E {{ λ v, Φ v ∗ at_boundary Λ1 }} -∗ link_in_state In1 -∗
-             WP (LkSE (Link.Expr1 e1)) @ pe; E {{ λ v, Φ v ∗ link_in_state Boundary }}) ∗
-    (∀ e2 Φ, WP e2 @ pe2; E {{ λ v, Φ v ∗ at_boundary Λ2 }} -∗ link_in_state In2 -∗
-             WP (LkSE (Link.Expr2 e2)) @ pe; E {{ λ v, Φ v ∗ link_in_state Boundary }})
+    (∀ e1 Φ, WP e1 @ ⟪p1, Ψ1⟫; E {{ λ v, Φ v ∗ at_boundary Λ1 }} -∗ link_in_state In1 -∗
+             WP (LkSE (Link.Expr1 e1)) @ ⟪link_prog p1 p2, Ψ⟫; E {{ λ v, Φ v ∗ link_in_state Boundary }}) ∗
+    (∀ e2 Φ, WP e2 @ ⟪p2, Ψ2⟫; E {{ λ v, Φ v ∗ at_boundary Λ2 }} -∗ link_in_state In2 -∗
+             WP (LkSE (Link.Expr2 e2)) @ ⟪link_prog p1 p2, Ψ⟫; E {{ λ v, Φ v ∗ link_in_state Boundary }})
   ).
 Proof using.
-  intros Hislink. iLöb as "IH". iModIntro. iSplitL.
+  intros Hcanlink. iLöb as "IH". iModIntro. iSplitL.
   (* Case 1: running Λ1 *)
   { iIntros (e1 Φ) "Hwp [Hb Hb2]".
     rewrite wp_unfold. rewrite /wp_pre.
@@ -421,11 +414,11 @@ Proof using.
 
       (* two cases: this is an external call of the linking module itself, or it
          is a call to a function of pe2 *)
-      destruct (penv_prog pe2 !! f) as [fn2|] eqn:Hf2.
+      destruct (p2 !! f) as [fn2|] eqn:Hf2.
 
       { (* call to a function of pe2 *)
-        assert (penv_prog pe !! f = Some (inr fn2)) as Hpef.
-        { rewrite is_link_prog lookup_union_r lookup_fmap. by rewrite Hf2. by rewrite Hf. }
+        assert (link_prog p1 p2 !! f = Some (inr fn2)) as Hpef.
+        { rewrite lookup_union_r lookup_fmap. by rewrite Hf2. by rewrite Hf. }
 
         (* administrative step CallS: Link.ExprCall ~> LinkRunFunction *)
         iApply wp_link_call; first done.
@@ -463,9 +456,9 @@ Proof using.
       inversion Hstep; simplify_eq. clear H4 H5.
       clear Hstep. rename H2 into Hstep.
       specialize (Hstep _ _ eq_refl).
-      rewrite is_link_prog proj1_prog_union in Hstep; [|apply Hislink].
+      rewrite proj1_prog_union in Hstep; [|apply Hcanlink].
       assert (¬ (∃ (K : cont Λ1) (fn_name : string) (arg : list val),
-             is_call e1 fn_name arg K ∧ penv_prog pe1 !! fn_name = None)) as HHHH.
+             is_call e1 fn_name arg K ∧ p1 !! fn_name = None)) as HHHH.
       { intros (?&?&?&?&?); eapply Hnocall; eauto. }
       specialize (Hstep HHHH Hred).
       destruct Hstep as (X1&Hstep&HX1).
@@ -512,11 +505,11 @@ Proof using.
 
       (* two cases: this is an external call of the linking module itself, or it
          is a call to a function of pe1 *)
-      destruct (penv_prog pe1 !! f) as [fn1|] eqn:Hf1.
+      destruct (p1 !! f) as [fn1|] eqn:Hf1.
 
       { (* call to a function of pe1 *)
-        assert (penv_prog pe !! f = Some (inl fn1)) as Hpef.
-        { rewrite is_link_prog lookup_union_l lookup_fmap. by rewrite Hf1. by rewrite Hf. }
+        assert (link_prog p1 p2 !! f = Some (inl fn1)) as Hpef.
+        { rewrite lookup_union_l lookup_fmap. by rewrite Hf1. by rewrite Hf. }
 
         (* administrative step CallS: Link.ExprCall ~> LinkRunFunction *)
         iApply wp_link_call; first done.
@@ -554,9 +547,9 @@ Proof using.
       inversion Hstep; simplify_eq. clear H4 H5.
       clear Hstep. rename H2 into Hstep.
       specialize (Hstep _ _ eq_refl).
-      rewrite is_link_prog proj2_prog_union in Hstep; [|apply Hislink].
+      rewrite proj2_prog_union in Hstep; [|apply Hcanlink].
       assert (¬ (∃ (K : cont Λ2) (fn_name : string) (arg : list val),
-             is_call e1 fn_name arg K ∧ penv_prog pe2 !! fn_name = None)) as HHHH.
+             is_call e1 fn_name arg K ∧ p2 !! fn_name = None)) as HHHH.
       { intros (?&?&?&?&?); eapply Hnocall; eauto. }
       specialize (Hstep HHHH Hred).
       destruct Hstep as (X1&Hstep&HX1).
@@ -565,44 +558,44 @@ Proof using.
       iDestruct "IH" as "[_ IH2]". iApply ("IH2" with "Hwp [$Hb $Hb1]"). } }
 Qed.
 
-Lemma wp_link_run1 pe1 pe2 pe E e1 Φ :
-  is_link_environ pe1 pe2 pe →
+Lemma wp_link_run1 p1 p2 Ψ1 Ψ2 Ψ E e1 Φ :
+  can_link p1 Ψ1 p2 Ψ2 Ψ →
   link_in_state In1 -∗
-  WP e1 @ pe1; E {{ λ v, Φ v ∗ at_boundary Λ1 }} -∗
-  WP LkSE (Link.Expr1 e1) @ pe; E {{ λ v, Φ v ∗ link_in_state Boundary }}.
+  WP e1 @ ⟪p1, Ψ1⟫; E {{ λ v, Φ v ∗ at_boundary Λ1 }} -∗
+  WP LkSE (Link.Expr1 e1) @ ⟪link_prog p1 p2, Ψ⟫; E {{ λ v, Φ v ∗ link_in_state Boundary }}.
 Proof using.
-  iIntros (Hislink) "Hlkst Hwp". iDestruct (wp_link_run_mut _ _ _ _ Hislink) as "[H _]".
+  iIntros (Hcanlink) "Hlkst Hwp". iDestruct (wp_link_run_mut _ _ _ _ _ _ Hcanlink) as "[H _]".
   iApply ("H" with "Hwp Hlkst").
 Qed.
 
-Lemma wp_link_run1' pe1 pe2 pe E e1 Φ Ψ :
-  is_link_environ pe1 pe2 pe →
+Lemma wp_link_run1' p1 p2 Ψ1 Ψ2 Ψ E e1 Φ Φ' :
+  can_link p1 Ψ1 p2 Ψ2 Ψ →
   link_in_state In1 -∗
-  WP e1 @ pe1; E {{ λ v, Φ v ∗ at_boundary Λ1 }} -∗
-  (∀ v, Φ v ∗ link_in_state Boundary -∗ Ψ v) -∗
-  WP LkSE (Link.Expr1 e1) @ pe; E {{ Ψ }}.
+  WP e1 @ ⟪p1, Ψ1⟫; E {{ λ v, Φ v ∗ at_boundary Λ1 }} -∗
+  (∀ v, Φ v ∗ link_in_state Boundary -∗ Φ' v) -∗
+  WP LkSE (Link.Expr1 e1) @ ⟪link_prog p1 p2, Ψ⟫; E {{ Φ' }}.
 Proof using.
   iIntros (?) "Hin Hwp HΦ". iApply (wp_wand with "[-HΦ]").
   { iApply (wp_link_run1 with "Hin Hwp"). }
   done.
 Qed.
 
-Lemma wp_link_run2 pe1 pe2 pe E e2 Φ :
-  is_link_environ pe1 pe2 pe →
+Lemma wp_link_run2 p1 p2 Ψ1 Ψ2 Ψ E e2 Φ :
+  can_link p1 Ψ1 p2 Ψ2 Ψ →
   link_in_state In2 -∗
-  WP e2 @ pe2; E {{ λ v, Φ v ∗ at_boundary Λ2 }} -∗
-  WP LkSE (Link.Expr2 e2) @ pe; E {{ λ v, Φ v ∗ link_in_state Boundary }}.
+  WP e2 @ ⟪p2, Ψ2⟫; E {{ λ v, Φ v ∗ at_boundary Λ2 }} -∗
+  WP LkSE (Link.Expr2 e2) @ ⟪link_prog p1 p2, Ψ⟫; E {{ λ v, Φ v ∗ link_in_state Boundary }}.
 Proof using.
-  iIntros (Hislink) "Hlkst Hwp". iDestruct (wp_link_run_mut _ _ _ _ Hislink) as "[_ H]".
+  iIntros (Hcanlink) "Hlkst Hwp". iDestruct (wp_link_run_mut _ _ _ _ _ _ Hcanlink) as "[_ H]".
   iApply ("H" with "Hwp Hlkst").
 Qed.
 
-Lemma wp_link_run2' pe1 pe2 pe E e2 Φ Ψ :
-  is_link_environ pe1 pe2 pe →
+Lemma wp_link_run2' p1 p2 Ψ1 Ψ2 Ψ E e2 Φ Φ' :
+  can_link p1 Ψ1 p2 Ψ2 Ψ →
   link_in_state In2 -∗
-  WP e2 @ pe2; E {{ λ v, Φ v ∗ at_boundary Λ2 }} -∗
-  (∀ v, Φ v ∗ link_in_state Boundary -∗ Ψ v) -∗
-  WP LkSE (Link.Expr2 e2) @ pe; E {{ Ψ }}.
+  WP e2 @ ⟪p2, Ψ2⟫; E {{ λ v, Φ v ∗ at_boundary Λ2 }} -∗
+  (∀ v, Φ v ∗ link_in_state Boundary -∗ Φ' v) -∗
+  WP LkSE (Link.Expr2 e2) @ ⟪link_prog p1 p2, Ψ⟫; E {{ Φ' }}.
 Proof using.
   iIntros (?) "Hin Hwp HΦ". iApply (wp_wand with "[-HΦ]").
   { iApply (wp_link_run2 with "Hin Hwp"). }
@@ -662,6 +655,37 @@ Proof using.
   simpl. iFrame. iApply ("Hwp" with "[-Hb2] Hb2"). iFrame.
 Qed.
 
+Lemma link_refines E p1 Ψ1 p2 Ψ2 Ψ :
+  can_link p1 Ψ1 p2 Ψ2 Ψ →
+  mprog_proto E p1 Ψ1 ⊔ mprog_proto E p2 Ψ2 ⊑ mprog_proto E (link_prog p1 p2) Ψ.
+Proof using.
+  iIntros (Hcanlink ? ? ?) "H".
+  rewrite /join /proto_join_join /proto_join /mprog_proto.
+  destruct (p1 !! s) as [fn|] eqn:HH1.
+  { destruct (p2 !! s) eqn:HH2; first exfalso.
+    { destruct Hcanlink. apply elem_of_dom_2 in HH1, HH2. set_solver. }
+    assert (link_prog p1 p2 !! s = Some (inl fn)) as HH3.
+    { rewrite /link_prog lookup_union_l lookup_fmap //.
+      rewrite HH1 //. rewrite HH2 //. (*TODO: lemma*) }
+    iApply (bi.or_elim with "H"); iIntros "H"; last done.
+    iDestruct "H" as (? ?) "H". rewrite HH3.
+    iExists _. iSplit; first done. iNext. iIntros "Hb".
+    iApply (wp_link_run_function1 with "Hb"); first done.
+    iNext. iIntros "Hin Hb".
+    iApply (wp_link_run1 with "Hin"). iApply ("H" with "Hb"). }
+  { destruct (p2 !! s) as [fn|] eqn:HH2.
+    2: { iExFalso. iApply (bi.or_elim with "H"); by iIntros. }
+    assert (link_prog p1 p2 !! s = Some (inr fn)) as HH3.
+    { rewrite /link_prog lookup_union_r lookup_fmap //.
+      rewrite HH2 //. rewrite HH1 //. (*TODO: lemma*) }
+    iApply (bi.or_elim with "H"); iIntros "H"; first done.
+    iDestruct "H" as (? ?) "H". rewrite HH3.
+    iExists _. iSplit; first done. iNext. iIntros "Hb".
+    iApply (wp_link_run_function2 with "Hb"); first done.
+    iNext. iIntros "Hin Hb".
+    iApply (wp_link_run2 with "Hin"). iApply ("H" with "Hb"). }
+Qed.
+
 End Linking_logic.
 
-Global Arguments is_link_environ {_ _ _ _ _ _ _ _ _ _ _} pe1 pe2 pe.
+Global Arguments can_link {_ _ _} _ _ {_ _ _} p1 Ψ1 p2 Ψ2 Ψ.
