theories/mlanguage/progenv.v
@@ -1,6 +1,6 @@
 From iris.proofmode Require Import base.
 From iris.base_logic.lib Require Import fancy_updates.
-From melocoton.mlanguage Require Export mlanguage.
+From melocoton.mlanguage Require Import mlanguage.
 From iris.prelude Require Import options.
 
 Record prog_environ {val} (Λ : mlanguage val) Σ := Penv {
@@ -11,4 +11,4 @@ Global Arguments Penv {_ _ _} _ _.
 Global Arguments penv_prog {_ _ _} _.
 Global Arguments penv_proto {_ _ _} _.
 
-Notation "⟪ p , T ⟫" := (Penv p T : prog_environ _ _).
+Notation "⟪ p , Ψ ⟫" := ({| penv_prog := p; penv_proto := Ψ |} : prog_environ _ _).
